# Proposition

> For isosceles triangles, the angles at the base are equal to one another, and if the equal sides are produced then the angles under the base will be equal to one another.

# Proof

![alt text](<../sources/The Elements/Screenshot 2025-12-12 at 9.40.05â€¯PM.png>)

Two parts to this:

1. $\angle ABC = \angle ACB$
2. $\angle FBC = \angle BCG$

First, let's say that $\angle ABC = \theta, \angle ACB = \phi$. Imagine you mirror $\triangle ABC$ into $\triangle A'B'C'$ such that now $\angle A'B'C' = \phi, \angle A'C'B' = \theta$. Since $AB = A'B'$ and $AC=A'C'$, by proposition 1.4, these two triangle must be equivalent and so $\theta = \phi$.

For the second part, first pick an arbitrary point $F$ along $BD$ and by proposition 1.3 we can find a point G s.t. $BF = CG$. Two triangles to look at $\triangle ACF, \triangle ABG$. We have that $AF = AG, AC=AB$ and the angle at $A$ are the same. By proposition 1.4, these 2 triangles are equivalent which means $\angle AFC = \angle AGB$ and that $CF = GB$. Again, by proposition 1.4, we have that $\triangle FBC = \triangle CBG$ which means $\angle FBC = \angle BCG$ $\square$.
